theories/lang/handler.v
@@ -25,187 +25,14 @@ Definition effect (op : string) := (LitV (LitStr op)).
 
 Definition rec_perform : val := (λ: "x", "x")%V.
 
-Notation "'perform:' op e" := (rec_perform (Do OS (Pair (Val (PairV (effect op) (LitV (LitInt 0)))) e%E)))
+Notation "'perform:' op e" := (rec_perform (Do MS (Pair (Val (PairV (effect op) (LitV (LitInt 0)))) e%E)))
   (at level 200, op at level 1, e at level 200,
    format "'[' 'perform:'  op  e ']'") : expr_scope.
 
-Notation "'performₘ:' op e" := (rec_perform (Do MS (Pair (Val (PairV (effect op) (LitV (LitInt 0)))) e%E)))
-  (at level 200, op at level 1, e at level 200,
-   format "'[' 'performₘ:'  op  e ']'") : expr_scope.
-
-Definition shallow_try_mode : val := (
-  λ: "e" "hos" "hms" "r",
-    shallow-try: "e" #() with
-      effect (λ: "x" "k", 
-          if: UnOp IsContOS "k" then
-            "hos" "x" "k"
-          else
-            "hms" "x" "k"
-      )
-    | return "r" 
-    end
-)%V.
-
-Arguments shallow_try_mode : simpl never.
-
-Definition ShallowTryMode (e : expr) (hos hms r : expr) : expr :=
-  shallow_try_mode (λ: <>, e)%E hos hms r.
-
-Definition ShallowTryModeV (e : expr) (hos hms r : expr) : expr :=
-  shallow_try_mode (λ: <>, e)%V hos hms r.
-
-Notation "'shallow-try-mode:' e 'with' 'effect-os' hos | 'effect-ms' hms | 'return' r 'end'" :=
-  (ShallowTryMode e hos hms r)
-  (e, hos, hms, r at level 200, only parsing) : expr_scope.
-
-Definition deep_try_mode : val := (
-    rec: "H" "e" "hos" "hms" "r" := 
-      ShallowTryMode ("e" #())
-        (λ: "x" "k", "hos" "x" (λ: "y", "H" (λ: <>, "k" "y") "hos" "hms" "r"))
-        (λ: "x" "k", "hms" "x" (λ: "y", "H" (λ: <>, "k" "y") "hos" "hms" "r"))
-        "r"
-)%V.
-
-Arguments deep_try_mode : simpl never.
-
-Definition DeepTryMode (e : expr) (hos hms r : expr) : expr :=
-  deep_try_mode (λ: <>, e)%E hos hms r.
-
-Definition DeepTryModeV (e : expr) (hos hms r : expr) : expr :=
-  deep_try_mode (λ: <>, e)%V hos hms r.
-
-Notation "'deep-try-mode:' e 'with' 'effect-os' hos | 'effect-ms' hms | 'return' r 'end'" :=
-  (DeepTryMode e hos hms r)
-  (e, hos, hms, r at level 200, only parsing) : expr_scope.
-
-
-Definition shallow_handler_mode `{irisGS eff_lang Σ}
-  (E : coPset)
-  (Ψ1 : iEff Σ)
-  (Ψ2 : iEff Σ)
-  (Φ : val -d> iPropO Σ)
-  (hos hms r : val)
-  (Ψ1' : iEff Σ)
-  (Ψ2' : iEff Σ)
-  (Φ' : val -d> iPropO Σ) : iProp Σ :=
-
-  (* Correctness of the return branch. *)
-  (∀ (y : val), Φ y -∗ EWP r y @ E <| Ψ1' |> {| Ψ2' |} {{ Φ' }}) ∧
-
-  (* Correctness of the effect one-shot branch. *)
-  (∀ (v k : val),
-     iEff_car (upcl OS Ψ1) v (λ w, EWP k w @ E <| Ψ1 |> {| Ψ2 |} {{ Φ }}) -∗
-       EWP hos v k @ E <| Ψ1' |> {| Ψ2' |} {{ Φ' }}) ∧
-
-  (* Correctness of the effect multi-shot branch. *)
-  (∀ (v k : val),
-     iEff_car (upcl MS Ψ2) v (λ w, EWP k w @ E <| Ψ1 |> {| Ψ2 |} {{ Φ }}) -∗
-       EWP hms v k @ E <| Ψ1' |> {| Ψ2' |} {{ Φ' }}).
-
-Lemma ewp_try_with_mode `{heapGS Σ} E e Ψ1 Ψ2 Φ (hos hms r : val) Ψ1' Ψ2' Φ' : 
-  EWP e @ E <| Ψ1 |> {| Ψ2 |} {{ Φ }} -∗
-    shallow_handler_mode E Ψ1 Ψ2 Φ hos hms r Ψ1' Ψ2' Φ' -∗
-      EWP (ShallowTryModeV e hos hms r) @ E <| Ψ1' |> {| Ψ2' |} {{ Φ' }}.
-Proof.
-  iIntros "He H". rewrite /ShallowTryModeV /shallow_try_mode /shallow_handler_mode. 
-  ewp_pure_steps. 
-  iApply (ewp_try_with with "[He] [H]").
-  { ewp_pure_steps. iApply "He". }
-  iSplit; last iSplit.
-  - iDestruct "H" as "[$ _]". 
-  - iIntros (v k) "(%N & %l & ->) HΨ1". 
-    iDestruct "H" as "[_ [H _]]". 
-    ewp_pure_steps; first done. ewp_pure_steps.
-    by iApply "H". 
-  - iIntros (v k) "(%N & ->) HΨ1". 
-    iDestruct "H" as "[_ [_ H]]". 
-    ewp_pure_steps; first done. ewp_pure_steps.
-    by iApply "H". 
-Qed.
-
-Notation deep_handler_mode_type Σ :=
-  (coPset -d> iEff Σ -d> iEff Σ -d> (val -d> iPropO Σ) 
-         -d> val -d> val -d> val 
-         -d> iEff Σ -d> iEff Σ -d> (val -d> iPropO Σ) -d> iPropO Σ) (only parsing).
-
-Definition deep_handler_mode_pre `{irisGS eff_lang Σ} :
-  deep_handler_mode_type Σ → deep_handler_mode_type Σ :=
-  (λ deep_handler_mode E Ψ1 Ψ2 Φ hos hms r Ψ1' Ψ2' Φ', 
-
-  (* Correctness of the return branch. *)
-  (∀ (y : val), Φ y -∗ EWP r y @ E <| Ψ1' |> {| Ψ2' |} {{ Φ' }}) ∧
-
-  (* Correctness of the effect one-shot branch. *)
-  (∀ (v k : val),
-     iEff_car (upcl OS Ψ1) v (λ w, 
-      ∀ Ψ1'' Ψ2'' Φ'',
-        ▷ deep_handler_mode E Ψ1 Ψ2 Φ hos hms r Ψ1'' Ψ2'' Φ'' -∗
-        EWP k w @ E <| Ψ1'' |> {| Ψ2'' |} {{ Φ'' }}) -∗
-       EWP hos v k @ E <| Ψ1' |> {| Ψ2' |} {{ Φ' }}) ∧
-
-  (* Correctness of the effect multi-shot branch. *)
-  (∀ (v k : val),
-     iEff_car (upcl MS Ψ2) v (λ w, 
-      ∀ Ψ1'' Ψ2'' Φ'',
-        ▷ deep_handler_mode E Ψ1 Ψ2 Φ hos hms r Ψ1'' Ψ2'' Φ'' -∗
-        EWP k w @ E <| Ψ1'' |> {| Ψ2'' |} {{ Φ'' }}) -∗
-       EWP hms v k @ E <| Ψ1' |> {| Ψ2' |} {{ Φ' }}))%I.
-
-Local Instance deep_handler_mode_pre_contractive `{heapGS Σ} : Contractive deep_handler_mode_pre.
-Proof.
-  rewrite /deep_handler_mode_pre => n deep deep' Hne E Ψ1 Ψ2 Φ h r Ψ1' Ψ2' Φ'.
-  repeat (f_contractive || f_equiv). intros ?; simpl.
-  repeat (f_contractive || f_equiv); apply Hne.
-Qed.
-Definition deep_handler_mode `{heapGS Σ} := fixpoint deep_handler_mode_pre.
-Arguments deep_handler_mode _ _%ieff _%ieff _%I _%V %V _%V _%ieff _%ieff _%I.
-
-Global Lemma deep_handler_mode_unfold `{heapGS Σ} E Ψ1 Ψ2 Φ hos hms r Ψ1' Ψ2' Φ' :
-  deep_handler_mode E Ψ1 Ψ2 Φ hos hms r Ψ1' Ψ2' Φ' ⊣⊢
-    deep_handler_mode_pre deep_handler_mode E Ψ1 Ψ2 Φ hos hms r Ψ1' Ψ2' Φ'.
-Proof.
-  by apply (fixpoint_unfold deep_handler_mode_pre).
-Qed.
-
-Lemma ewp_deep_try_with_mode `{heapGS Σ} E e Ψ1 Ψ2 Φ (hos hms r : val) Ψ1' Ψ2' Φ' : 
-  EWP e @ E <| Ψ1 |> {| Ψ2 |} {{ Φ }} -∗
-    deep_handler_mode E Ψ1 Ψ2 Φ hos hms r Ψ1' Ψ2' Φ' -∗
-      EWP (DeepTryModeV e hos hms r) @ E <| Ψ1' |> {| Ψ2' |} {{ Φ' }}.
-Proof.
-  iIntros "He H". rewrite /DeepTryModeV /deep_try_mode.
-  iLöb as "IH" forall (e Ψ1' Ψ2' Φ'). ewp_pure_steps.
-  rewrite deep_handler_mode_unfold /deep_handler_mode_pre.
-  iApply (ewp_try_with_mode with "[He] [H]").
-  { ewp_pure_steps. iApply "He". }
-  iSplit; last iSplit.
-  - iDestruct "H" as "[$ _]". 
-  - iIntros (v k) "/= (%Φ'' & HΨ1 & HPost)". 
-    iDestruct "H" as "[_ [H _]]".
-    ewp_pure_steps. iApply "H". iExists Φ''. iFrame.
-    iIntros (w) "HΦ'' % % %Φ''' Hdeep".
-    do 3 ewp_value_or_step.
-    iApply ("IH" with "[HΦ'' HPost] Hdeep"); by iApply "HPost".
-  - iIntros (v k) "/= (%Φ'' & HΨ2 & #HPost)".
-    iDestruct "H" as "[_ [_ H]]".
-    ewp_pure_steps. iApply "H". iExists Φ''. iFrame.
-    iIntros (w) "!# HΦ'' % % %Φ''' Hdeep".
-    do 3 ewp_value_or_step.
-    iApply ("IH" with "[HΦ'' HPost] Hdeep"); by iApply "HPost".
-Qed.
-
 Definition lft_def : val := 
   (λ: "op'" "e", 
-     deep-try-mode: "e" #() with
-       effect-os (λ: "x" "k", 
-             let: "op" := Fst (Fst "x") in
-             let: "s" := Snd (Fst "x") in
-             let: "x" := Snd "x" in
-             if: "op" = "op'" then
-               "k" (Do OS ("op", "s" + #1, "x"))
-             else
-               "k" (Do OS ("op", "s", "x"))
-         )
-       | effect-ms (λ: "x" "k", 
+     deep-try: "e" #() with
+         effect (λ: "x" "k", 
              let: "op" := Fst (Fst "x") in
              let: "s" := Snd (Fst "x") in
              let: "x" := Snd "x" in
@@ -224,17 +51,8 @@ Notation "'lft:' op e" := (App (App (Val lft_def) (Val (effect op))) (Rec BAnon 
 
 Definition unlft_def : val := 
   (λ: "op'" "e", 
-     deep-try-mode: "e" #() with
-       effect-os (λ: "x" "k", 
-             let: "op" := Fst (Fst "x") in
-             let: "s" := Snd (Fst "x") in
-             let: "x" := Snd "x" in
-             if: "op" = "op'" then
-               "k" (Do OS ("op", "s" - #1, "x"))
-             else
-               "k" (Do OS ("op", "s", "x"))
-         )
-       | effect-ms (λ: "x" "k", 
+     deep-try: "e" #() with
+         effect (λ: "x" "k", 
              let: "op" := Fst (Fst "x") in
              let: "s" := Snd (Fst "x") in
              let: "x" := Snd "x" in
@@ -251,116 +69,121 @@ Notation "'unlft:' op e" := (App (App (Val unlft_def) (Val (effect op))) (Rec BA
   (at level 200, op at level 1, e at level 200,
    format "'[' 'unlft:'  op  e ']'") : expr_scope.
 
-Definition shandler : val := (
+Definition assert : val := (λ: "x", if: "x" then #() else #() #())%V.
+Notation "'assert:' e" := (assert e)%E
+  (at level 75, format "'[' 'assert:'  e ']'") : expr_scope.
+
+Definition shandler (m : mode) : val := (
   rec: "H" "e" "op'" "h" "r" :=
-    shallow_try_mode "e" 
-      (λ: "x" "k",
+    shallow-try: "e" #() with
+      effect (λ: "x" "k",
           let: "op" := Fst (Fst "x") in
           let: "s" := Snd (Fst "x") in
           let: "x" := Snd "x" in
           if: ("op" = "op'") && ("s" = #0) then
-            "h" "x" "k"
-          else
-            (λ: "y", "H" (λ: <>, "k" "y") "op'" "h" "r") (unlft_def "op'" (λ: <>, do: ("op", "s", "x")))
-      )%E
-      (λ: "x" "k",
-          let: "op" := Fst (Fst "x") in
-          let: "s" := Snd (Fst "x") in
-          let: "x" := Snd "x" in
-          if: ("op" = "op'") && ("s" = #0) then
-            "h" "x" "k"
+            "h" "x" (match m with
+                          OS => let: "l" := ref #true in 
+                                (λ: "x", assert: (Load "l") ;; "l" <- #false ;; "k" "x")%E
+                        | MS => "k"
+                        end)
           else
             (λ: "y", "H" (λ: <>, "k" "y") "op'" "h" "r") (unlft_def "op'" (λ: <>, doₘ: ("op", "s", "x")))
       )%E
-      "r"
+      | return "r"
+  end
 )%V.
 
 Arguments shandler : simpl never.
 
-Definition SHandler (e : expr) (op : operation) (h r : expr) : expr :=
-  shandler (λ: <>, e)%E (effect op) h r.
+Definition SHandler (m : mode) (e : expr) (op : operation) (h r : expr) : expr :=
+  shandler m (λ: <>, e)%E (effect op) h r.
 
-Definition SHandlerV (e : expr) (op : operation) (h r : expr) : expr :=
-  shandler (λ: <>, e)%V (effect op) h r.
+Definition SHandlerV (m : mode) (e : expr) (op : operation) (h r : expr) : expr :=
+  shandler m (λ: <>, e)%V (effect op) h r.
 
 Notation "'shandle:' e 'by' op '=>' h | 'ret' '=>' r 'end'" :=
-  (SHandler e%E op h%E r%E)
+  (SHandler OS e%E op h%E r%E)
   (e, op, h, r at level 200) : expr_scope.
 
-Definition handler : val := (
+Notation "'shandleₘ:' e 'by' op '=>' h | 'ret' '=>' r 'end'" :=
+  (SHandler MS e%E op h%E r%E)
+  (e, op, h, r at level 200) : expr_scope.
+
+Definition handler (m : mode) : val := (
   λ: "e" "op'" "h" "r",
-    deep_try_mode "e"
-      (λ: "x" "k", 
+    deep-try: "e" #() with
+      effect (λ: "x" "k", 
           let: "op" := Fst (Fst "x") in
           let: "s" := Snd (Fst "x") in
           let: "x" := Snd "x" in
           if: ("op" = "op'") && ("s" = #0) then
-            "h" "x" "k"
-          else
-            "k" (unlft_def "op'" (λ: <>, do: ("op", "s", "x")))
-      )
-      (λ: "x" "k", 
-          let: "op" := Fst (Fst "x") in
-          let: "s" := Snd (Fst "x") in
-          let: "x" := Snd "x" in
-          if: ("op" = "op'") && ("s" = #0) then
-            "h" "x" "k"
+            "h" "x" (match m with
+                        OS => let: "l" := ref #true in 
+                              (λ: "x", assert: (Load "l") ;; "l" <- #false ;; "k" "x")%E
+                      | MS => "k"
+                      end)
           else
             "k" (unlft_def "op'" (λ: <>, doₘ: ("op", "s", "x")))
       )
-      "r" 
+    | return "r" 
+    end
 )%V.
             
 Arguments handler : simpl never.
 
-Definition Handler (e : expr) (op : operation) (h r : expr) : expr :=
-  handler (λ: <>, e)%E (effect op) h r.
+Definition Handler (m : mode) (e : expr) (op : operation) (h r : expr) : expr :=
+  handler m (λ: <>, e)%E (effect op) h r.
 
-Definition HandlerV (e : expr) (op : operation) (h r : expr) : expr :=
-  handler (λ: <>, e)%V (effect op) h r.
+Definition HandlerV (m : mode) (e : expr) (op : operation) (h r : expr) : expr :=
+  handler m (λ: <>, e)%V (effect op) h r.
 
 Notation "'handle:' e 'by' op '=>' h | 'ret' '=>' r 'end'" :=
-  (Handler e%E op h%E r%E)
+  (Handler OS e%E op h%E r%E)
   (e, op, h, r at level 200) : expr_scope.
 
-Definition handler2 : val := (
+Notation "'handleₘ:' e 'by' op '=>' h | 'ret' '=>' r 'end'" :=
+  (Handler MS e%E op h%E r%E)
+  (e, op, h, r at level 200) : expr_scope.
+
+Definition handler2 (m : mode) : val := (
   λ: "e" "op1" "h1" "op2" "h2" "r",
-    deep_try_mode "e"
-      (λ: "x" "k", 
-          let: "op" := Fst (Fst "x") in
-          let: "s" := Snd (Fst "x") in
-          let: "x" := Snd "x" in
-          if: ("op" = "op1") && ("s" = #0) then
-            "h1" "x" "k"
-          else
-            if: ("op" = "op2") && ("s" = #0) then
-              "h2" "x" "k"
+    deep-try: "e" #() with
+        effect (λ: "x" "k", 
+            let: "op" := Fst (Fst "x") in
+            let: "s" := Snd (Fst "x") in
+            let: "x" := Snd "x" in
+            if: ("op" = "op1") && ("s" = #0) then
+                "h1" "x" (match m with
+                            OS => let: "l" := ref #true in 
+                                  (λ: "x", assert: (Load "l") ;; "l" <- #false ;; "k" "x")%E
+                          | MS => "k"
+                          end)
             else
-              "k" (unlft_def "op2" (λ: <>, unlft_def "op1" (λ: <>, do: ("op", "s", "x"))))
-      )
-      (λ: "x" "k", 
-          let: "op" := Fst (Fst "x") in
-          let: "s" := Snd (Fst "x") in
-          let: "x" := Snd "x" in
-          if: ("op" = "op1") && ("s" = #0) then
-            "h1" "x" "k"
-          else
-            if: ("op" = "op2") && ("s" = #0) then
-              "h2" "x" "k"
-            else
-              "k" (unlft_def "op2" (λ: <>, unlft_def "op1" (λ: <>, doₘ: ("op", "s", "x"))))
-      )
-      "r" 
+              if: ("op" = "op2") && ("s" = #0) then
+                "h2" "x" (match m with
+                            OS => let: "l" := ref #true in 
+                                  (λ: "x", assert: (Load "l") ;; "l" <- #false ;; "k" "x")%E
+                          | MS => "k"
+                          end)
+              else
+                "k" (unlft_def "op2" (λ: <>, unlft_def "op1" (λ: <>, doₘ: ("op", "s", "x"))))
+        )
+        | return "r" 
+    end
 )%V.
             
 Arguments handler2 : simpl never.
 
-Definition Handler2 (e : expr) (op1 op2 : operation) (h1 h2 r : expr) : expr :=
-  handler2 (λ: <>, e)%E (effect op1) h1 (effect op2) h2 r.
+Definition Handler2 (m : mode) (e : expr) (op1 op2 : operation) (h1 h2 r : expr) : expr :=
+  handler2 m (λ: <>, e)%E (effect op1) h1 (effect op2) h2 r.
 
-Definition Handler2V (e : expr) (op1 op2 : operation) (h1 h2 r : expr) : expr :=
-  handler2 (λ: <>, e)%V (effect op1) h1 (effect op2) h2 r.
+Definition Handler2V (m : mode) (e : expr) (op1 op2 : operation) (h1 h2 r : expr) : expr :=
+  handler2 m (λ: <>, e)%V (effect op1) h1 (effect op2) h2 r.
 
 Notation "'handle2:' e 'by' op1 '=>' h1 | op2 '=>' h2 | 'ret' '=>' r 'end'" :=
-  (Handler2 e%E op1 op2 h1%E h2%E r%E)
+  (Handler2 OS e%E op1 op2 h1%E h2%E r%E)
+  (e, op1, h1, op2, h2, r at level 200) : expr_scope.
+
+Notation "'handle2ₘ:' e 'by' op1 '=>' h1 | op2 '=>' h2 | 'ret' '=>' r 'end'" :=
+  (Handler2 MS e%E op1 op2 h1%E h2%E r%E)
   (e, op1, h1, op2, h2, r at level 200) : expr_scope.
