theories/logic/sem_sig.v
@@ -18,33 +18,29 @@ From haffel.logic Require Import sem_def.
 From haffel.logic Require Import mode.
 
 Lemma sem_sig_to_ieff {Σ} (σ σ' : sem_sig Σ) : 
-    σ ≤S σ' -∗ iEff_le σ.2 σ'.2.
-Proof. iIntros "[_ $]". Qed.
+    σ ≤S σ' -∗ iEff_le σ σ'.
+Proof. iIntros "H". rewrite /sig_le. iApply "H". Qed.
 
 (* Single Variable Universally Quantified Effect Signatures *)
 (* Effect Signature *)
 Definition sem_sig_eff {Σ} m (A B : sem_ty Σ -d> sem_ty Σ) : sem_sig Σ :=
-  (m, >> (α : sem_ty Σ) (a : val) >> ! a {{ ▷ (A α a) }}; 
-      << (b : val)                << ? b {{ ▷ (B α b) }} @m)%ieff.
+  (>> (α : sem_ty Σ) (a : val) >> ! a {{ ▷ (A α a) }}; 
+   << (b : val)                << ? b {{ ▷ (B α b) }} @m)%ieff.
 
-Lemma sem_sig_eff_unfold_1 {Σ} m (A B : sem_ty Σ → sem_ty Σ) :
-  (sem_sig_eff m A B).1 ≡ m.
-Proof. by rewrite /sem_sig_eff. Qed.
-
-Lemma sem_sig_eff_unfold_2 {Σ} m (A B : sem_ty Σ -d> sem_ty Σ) :
-  (sem_sig_eff m A B).2 ≡
+Lemma sem_sig_eff_unfold {Σ} m (A B : sem_ty Σ -d> sem_ty Σ) :
+  (sem_sig_eff m A B) ≡
     (>> (α : sem_ty Σ) (a : val) >> ! a {{ ▷ (A α a) }}; 
      << (b : val)                << ? b {{ ▷ (B α b) }} @m)%ieff.
 Proof. by rewrite /sem_sig_eff. Qed.
 
 Lemma sem_sig_eff_unfold_iEff {Σ} m (A B : sem_ty Σ -d> sem_ty Σ) v Φ:
-  iEff_car (sem_sig_eff m A B).2 v Φ ⊣⊢
+  iEff_car (sem_sig_eff m A B) v Φ ⊣⊢
     iEff_car (>> (α : sem_ty Σ) (a : val) >> ! a {{ ▷ (A α a) }}; 
               << (b : val)                << ? b {{ ▷ (B α b) }} @m)%ieff v Φ.
 Proof. done. Qed.
 
 Lemma sem_sig_eff_eq {Σ} m A B v Φ :
-  iEff_car (@sem_sig_eff Σ m A B).2 v Φ ⊣⊢
+  iEff_car (@sem_sig_eff Σ m A B) v Φ ⊣⊢
     (∃ α a, ⌜ a = v ⌝ ∗ ▷ (A α a) ∗ 
                         □? m (∀ b, ▷ (B α b) -∗ Φ b))%I.
 Proof. 
@@ -54,7 +50,7 @@ Qed.
 
 (* The sem_sig_eff protocol is monotonic. *)
 Global Instance sem_sig_eff_mono_prot {Σ} A B :
-  MonoProt (@sem_sig_eff Σ OS A B).2.
+  MonoProt (@sem_sig_eff Σ OS A B).
 Proof.
   constructor. iIntros (???) "HΦ'".
   rewrite !sem_sig_eff_eq /=.
@@ -65,7 +61,7 @@ Qed.
 
 (* The sem_sig_eff protocol is persistently monotonic. *)
 Global Instance sem_sig_eff_pers_mono_prot {Σ} A B :
-  PersMonoProt (@sem_sig_eff Σ MS A B).2.
+  PersMonoProt (@sem_sig_eff Σ MS A B).
 Proof.
   constructor. iIntros (???) "#HΦ'".
   rewrite !sem_sig_eff_eq. simpl.
@@ -75,12 +71,12 @@ Proof.
 Qed.
 
 Lemma upcl_sem_sig_eff {Σ} m A B v Φ :
-  iEff_car (upcl m (@sem_sig_eff Σ m A B).2) v Φ ⊣⊢
+  iEff_car (upcl m (@sem_sig_eff Σ m A B)) v Φ ⊣⊢
     (∃ α a, ⌜ a = v ⌝ ∗ ▷ (A α a) ∗ 
                         □? m (∀ b, ▷ (B α b) -∗ Φ b))%I.
 Proof.
   assert (Hequiv:
-    iEff_car (upcl m (sem_sig_eff m A B).2) v Φ ≡ iEff_car (sem_sig_eff m A B).2 v Φ).
+    iEff_car (upcl m (sem_sig_eff m A B)) v Φ ≡ iEff_car (sem_sig_eff m A B) v Φ).
   { f_equiv. apply non_dep_fun_equiv. destruct m; [by rewrite upcl_id|by rewrite pers_upcl_id]. }
   rewrite Hequiv. by apply sem_sig_eff_eq.
 Qed.
@@ -93,27 +89,23 @@ Notation "'∀S:' α , τ ⇒ κ | m " := (sem_sig_eff m (λ α, τ%T) (λ α, �
 
 (* Effect Signature *)
 Definition sem_sig_prot {Σ} {TT : tele} m (A B : TT → sem_ty Σ) : sem_sig Σ :=
-  (m, >>.. (αs : TT) >> >> (a : val) >>  ! a {{ ▷ (A αs a) }}; 
-                        << (b : val) <<  ? b {{ ▷ (B αs b) }} @m)%ieff.
+  (>>.. (αs : TT) >> >> (a : val) >>  ! a {{ ▷ (A αs a) }}; 
+                     << (b : val) <<  ? b {{ ▷ (B αs b) }} @m)%ieff.
 
-Lemma sem_sig_prot_unfold_1 {Σ} {TT : tele} m (A B : TT → sem_ty Σ) :
-  (sem_sig_prot m A B).1 ≡ m. 
-Proof. rewrite /sem_sig_prot //. Qed.
-
-Lemma sem_sig_prot_unfold_2 {Σ} {TT : tele} m (A B : TT → sem_ty Σ) :
-  (sem_sig_prot m A B).2 ≡ 
+Lemma sem_sig_prot_unfold {Σ} {TT : tele} m (A B : TT → sem_ty Σ) :
+  (sem_sig_prot m A B) ≡ 
   (>>.. (αs : TT) >> >> (a : val) >> ! a {{ ▷ (A αs a) }}; 
                      << (b : val) << ? b {{ ▷ (B αs b) }} @m)%ieff.
 Proof. rewrite /sem_sig_prot //. Qed.
 
 Lemma sem_sig_prot_unfold_iEff {Σ} {TT : tele} m (A B : TT → sem_ty Σ) v Φ:
-  iEff_car (sem_sig_prot m A B).2 v Φ ⊣⊢
+  iEff_car (sem_sig_prot m A B) v Φ ⊣⊢
     iEff_car (>>.. (αs : TT) >> >> (a : val) >> ! a {{ ▷ (A αs a) }}; 
                                 << (b : val) << ? b {{ ▷ (B αs b) }} @m)%ieff v Φ.
 Proof. done. Qed.
 
 Lemma sem_sig_prot_eq {Σ} {TT : tele} m A B v Φ :
-  iEff_car (@sem_sig_prot Σ TT m A B).2 v Φ ⊣⊢
+  iEff_car (@sem_sig_prot Σ TT m A B) v Φ ⊣⊢
     (∃.. αs, ∃ a, ⌜ a = v ⌝ ∗ ▷ (A αs a) ∗ 
                              □? m (∀ b, ▷ (B αs b) -∗ Φ b))%I.
 Proof. 
@@ -123,7 +115,7 @@ Qed.
 
 (* The sem_sig_prot protocol is monotonic. *)
 Global Instance sem_sig_prot_mono_prot {Σ} {TT : tele} A B :
-  MonoProt (@sem_sig_prot Σ TT OS A B).2.
+  MonoProt (@sem_sig_prot Σ TT OS A B).
 Proof.
   constructor. iIntros (???) "HΦ'".
   rewrite !sem_sig_prot_eq /=.
@@ -134,7 +126,7 @@ Qed.
 
 (* The sem_sig_eff protocol is persistently monotonic. *)
 Global Instance sem_sig_prot_pers_mono_prot {Σ} {TT : tele} A B :
-  PersMonoProt (@sem_sig_prot Σ TT MS A B).2.
+  PersMonoProt (@sem_sig_prot Σ TT MS A B).
 Proof.
   constructor. iIntros (???) "#HΦ'".
   rewrite !sem_sig_prot_eq. simpl.
@@ -144,12 +136,12 @@ Proof.
 Qed.
 
 Lemma upcl_sem_sig_prot {Σ} {TT : tele} m A B v Φ :
-  iEff_car (upcl m (@sem_sig_prot Σ TT m A B).2) v Φ ⊣⊢
+  iEff_car (upcl m (@sem_sig_prot Σ TT m A B)) v Φ ⊣⊢
     (∃.. αs, ∃ a, ⌜ a = v ⌝ ∗ ▷ (A αs a) ∗ 
                               □? m (∀ b, ▷ (B αs b) -∗ Φ b))%I.
 Proof.
   assert (Hequiv:
-    iEff_car (upcl m (sem_sig_prot m A B).2) v Φ ≡ iEff_car (sem_sig_prot m A B).2 v Φ).
+    iEff_car (upcl m (sem_sig_prot m A B)) v Φ ≡ iEff_car (sem_sig_prot m A B) v Φ).
   { f_equiv. apply non_dep_fun_equiv. destruct m; [by rewrite upcl_id|by rewrite pers_upcl_id]. }
   rewrite Hequiv. by apply sem_sig_prot_eq.
 Qed.
@@ -170,7 +162,7 @@ Notation "'∀S..:' tt , κ ⇒ ι | m" :=
 
 (* Eval cbn in (∀S.: (α : sem_ty Σ), (sem_ty_prod α α) ⇒ (sem_ty_cpy α) | OS)%S. *)
 
-Definition sem_sig_os {Σ} (σ : sem_sig Σ) : sem_sig Σ := (σ.1, upcl OS σ.2).
+Definition sem_sig_os {Σ} (σ : sem_sig Σ) : sem_sig Σ := (upcl OS σ).
 Notation "¡ σ" := (sem_sig_os σ) (at level 10) : sem_sig_scope.
 
 (* One-Shot Signatures *)
@@ -181,10 +173,10 @@ Definition mono_prot {Σ} (Ψ : iEff Σ) : iProp Σ :=
               (iEff_car Ψ v Φ) -∗ (iEff_car Ψ v Φ').
 
 Class OSSig {Σ} (σ : sem_sig Σ) := { 
-  monotonic_prot : (⊢ mono_prot σ.2)
+  monotonic_prot : (⊢ mono_prot σ)
 }.
 
-Lemma mono_prot_os_sig {Σ} (σ : sem_sig Σ) `{!MonoProt σ.2 }: OSSig σ.
+Lemma mono_prot_os_sig {Σ} (σ : sem_sig Σ) `{!MonoProt σ }: OSSig σ.
 Proof. inv MonoProt0. constructor. iIntros (v Φ Φ') "HPost Hσ". 
        iApply (monotonic_prot0 v Φ Φ' with "HPost Hσ"). 
 Qed.
@@ -212,17 +204,15 @@ Qed.
 (* Sub-Typing on Signatures *)
 
 Lemma sig_le_refl {Σ} (σ : sem_sig Σ) : ⊢ σ ≤S σ.
-Proof. iSplit;[iApply mode_le_refl|iApply iEff_le_refl]. Qed.
+Proof. iApply iEff_le_refl. Qed.
 
 Lemma sig_le_trans {Σ} (σ₁ σ₂ σ₃: sem_sig Σ) : 
     σ₁ ≤S σ₂ -∗
     σ₂ ≤S σ₃ -∗
     σ₁ ≤S σ₃. 
 Proof. 
-  iIntros "[#Hm₁₂ #Hp₁₂] [#Hm₂₃ #Hp₂₃]"; rewrite /sig_le /tc_opaque. 
-  iSplitL.
-  - by iApply mode_le_trans.
-  - iApply iEff_le_trans; [iApply "Hp₁₂"|iApply "Hp₂₃"].
+  iIntros "#Hp₁₂ #Hp₂₃"; rewrite /sig_le /tc_opaque. 
+  iApply iEff_le_trans; [iApply "Hp₁₂"|iApply "Hp₂₃"].
 Qed.
 
 Lemma sig_le_eff {Σ} m₁ m₂ (ι₁ ι₂ κ₁ κ₂ : sem_ty Σ → sem_ty Σ) :
@@ -231,8 +221,7 @@ Lemma sig_le_eff {Σ} m₁ m₂ (ι₁ ι₂ κ₁ κ₂ : sem_ty Σ → sem_ty 
   □ (∀ α, (κ₂ α) ≤T (κ₁ α)) -∗
   (∀S: α , ι₁ α ⇒ κ₁ α | m₁) ≤S (∀S: α , ι₂ α ⇒ κ₂ α | m₂).
 Proof.
-  iIntros "#Hmle #Hι₁₂ #Hκ₂₁". iSplitL.
-  { by rewrite !sem_sig_eff_unfold_1 /=. }
+  iIntros "#Hmle #Hι₁₂ #Hκ₂₁". 
   iIntros (v Φ) "!#".
   rewrite !sem_sig_eff_eq.
   iIntros "(%α & %w & <- & Hι₁ & HκΦ₁)".
@@ -256,8 +245,7 @@ Lemma sig_le_prot {Σ} {TT : tele} m₁ m₂ (ι₁ ι₂ κ₁ κ₂ : TT → s
   □ (∀.. α, (κ₂ α) ≤T (κ₁ α)) -∗
   (∀S..: α , ι₁ α ⇒ κ₁ α | m₁) ≤S (∀S..: α , ι₂ α ⇒ κ₂ α | m₂).
 Proof.
-  iIntros "#Hmle #Hι₁₂ #Hκ₂₁". iSplitL.
-  { by rewrite !sem_sig_prot_unfold_1 /=. }
+  iIntros "#Hmle #Hι₁₂ #Hκ₂₁". 
   iIntros (v Φ) "!#".
   rewrite !sem_sig_prot_eq.
   iIntros "(%α & %w & <- & Hι₁ & HκΦ₁)".
@@ -278,7 +266,7 @@ Qed.
 Lemma sig_le_os_intro {Σ} (σ : sem_sig Σ) :
   ⊢ σ ≤S (¡ σ).
 Proof.
-  rewrite /sem_sig_os. iSplit; [iApply mode_le_refl|].
+  rewrite /sem_sig_os. 
   iIntros (v Φ) "!# Hσ". simpl.
   iExists Φ. iFrame. iIntros "% $".
 Qed.
@@ -286,7 +274,7 @@ Qed.
 Lemma sig_le_os_elim {Σ} (σ : sem_sig Σ) `{! OSSig σ} :
   ⊢ ¡ σ ≤S σ.
 Proof.
-  rewrite /sem_sig_os. iSplit; [iApply mode_le_refl|].
+  rewrite /sem_sig_os. 
   iIntros (v Φ) "!# (%Φ' & Hσ & Himp)". simpl.
   destruct OSSig0 as []. 
   iApply (monotonic_prot0 with "Himp Hσ").
@@ -295,7 +283,7 @@ Qed.
 Lemma sig_le_os_comp {Σ} (σ σ' : sem_sig Σ) :
   σ ≤S σ' -∗ (¡ σ) ≤S (¡ σ').
 Proof.
-  iIntros "[#Hlem #Hleσ]". 
-  iSplitL "Hlem"; first done.
+  iIntros "#Hleσ". 
+  rewrite /sig_le /sem_sig_os /tc_opaque.
   by iApply iEff_le_upcl.
 Qed.
